Incremental/Busy.lean
@@ -8,14 +8,14 @@ variable
   (ℭ : BuildConfig)
   (J : Type) [Input ℭ J]
 
-public def Busy {c : (Type → Type) → Type 1} (cId : c Id) :
-    Build c ℭ J where
+public def Busy {c : (Type → Type) → Type 1} (cId : c Id) (tasks : Tasks c ℭ) :
+    Build c ℭ J tasks where
   cId := cId
   σ := J
   init := id
   inputs := Input.get
   set i v := modify fun store => Input.set store i v
-  build tasks q store :=
-    (Subtype.mk (compute cId tasks (Input.get store) q) rfl, store)
+  build q store :=
+    (⟨compute cId tasks (Input.get store) q, rfl⟩, store)
 
 end Incremental
